iris/ProofSysLinkTails.v
@@ -1099,6 +1099,9 @@ Section ProofSysLinkTails.
     is_lock gk d_lock "virtio_disk"%string (disk_res gd pd pav pu) -∗
     bslots 3 -∗
     log_opS g (S u) Sb -∗
+    (* the transaction token beside the budget: this tail runs iupdate and
+       then end_op, which takes the whole [log_op] (durable-disk lane A) *)
+    log_tx g -∗
     (pa_stk sp0 1) ↦₈[KT1] (m !!! Regidx Rra : mword 64) -∗
     (pa_stk sp0 2) ↦₈[KT1] (m !!! Regidx Rs0 : mword 64) -∗
     (pa_stk sp0 3) ↦₈[KT1] (m !!! Regidx Rs1 : mword 64) -∗
@@ -1128,7 +1131,7 @@ Section ProofSysLinkTails.
            Hlkempty Heb Hsp0 HMsp HMthr HMs1 Hal Hncd.
     iIntros "Hcg Hown #Htext #Hdata Hpc #Hpe #Hbio #Hlog Hseam Hgen #Hitab #Hitinv
               #Hesck #Hireg #Hropen #Hslkk Hkeep Hru Hshr #Hshotc Hilink Htoken Hsbb Hsbi #Hbmres Hpid
-              #Hprocs #Hdev #Hgeo #Hdlk Hbsl Hop Hf1 Hf2 Hf3 Hf4 HbN HbW HbO
+              #Hprocs #Hdev #Hgeo #Hdlk Hbsl Hop Htx Hf1 Hf2 Hf3 Hf4 HbN HbW HbO
               Hcont".
     iDestruct (cpu_own_eb_agree with "Hcg Hown") as %Hb. cbn in Hb.
     (* ===== +0xf4 c.mv a0,s1 ===== *)
@@ -1496,10 +1499,10 @@ Section ProofSysLinkTails.
               with "Hcg Hown [] [] Htext Hdata Hpc Hpe Hbio Hlog Hitab Hitinv
                     Hesck Hireg Hropen Hslkk Hslkd Hdep Hidev Hiinum Hivalid
                     Hload Hshot' Hfrz [$Hkeep $Hru] Hsbb Hsbi Hbmres Hpid Hprocs Hdev Hgeo
-                    Hdlk Hbsl [Hop]").
+                    Hdlk Hbsl [Hop Htx]").
     { rewrite Heb /trap_csrs_ext. done. }
     { rewrite Heb /cpu_claim_ext. done. }
-    { rewrite /log_op. iExists (Sb ∪ {[IBLOCK inum inodestart]}). iExact "Hop". }
+    { iApply (log_opS_op with "Hop Htx"). }
     iIntros (CID12 Hq12 mup n2)
       "%Hcsup Hcg Hown _ _ Hpc Hpid Hsbb Hsbi Hbsl %Hn2
        Hop Hislot".
@@ -1772,6 +1775,9 @@ Section ProofSysLinkTails.
     is_lock gk d_lock "virtio_disk"%string (disk_res gd pd pav pu) -∗
     bslots 3 -∗
     log_opSe g n Sb e0 -∗
+    (* the transaction token beside the budget: this tail reaches end_op,
+       which takes the whole [log_op] (durable-disk lane A) *)
+    log_tx g -∗
     (pa_stk sp0 1) ↦₈[KT1] (m !!! Regidx Rra : mword 64) -∗
     (pa_stk sp0 2) ↦₈[KT1] (m !!! Regidx Rs0 : mword 64) -∗
     (pa_stk sp0 3) ↦₈[KT1] (m !!! Regidx Rs1 : mword 64) -∗
@@ -1803,7 +1809,7 @@ Section ProofSysLinkTails.
     iIntros "Hcg Hown #Htext #Hdata Hpc #Hpe #Hbio #Hlog Hseam Hgen #Hitab #Hitinv
               #Hesck #Hescd #Hireg #Hropen #Hslkk #Hslkd0 Hkeep Hru Hshr #Hshotc Hilink Htoken Hslkd
               Hdep Hidev Hiinum Hivalid Hload #Hshotd Hfrz Hkeepd Hrud Hsbb Hsbi
-              #Hbmres Hpid #Hprocs #Hdev #Hgeo #Hdlk Hbsl Hop Hf1 Hf2 Hf3 Hf4
+              #Hbmres Hpid #Hprocs #Hdev #Hgeo #Hdlk Hbsl Hop Htx Hf1 Hf2 Hf3 Hf4
               HbN HbW HbO Hcont".
     iDestruct (cpu_own_eb_agree with "Hcg Hown") as %Hb. cbn in Hb.
     (* ===== +0xee c.mv a0,s2 ===== *)
@@ -1899,7 +1905,7 @@ Section ProofSysLinkTails.
               Hlkempty Heb Hsp0 Hupsp Hupthr Hups1 Hal Hncd
               with "Hcg Hown Htext Hdata Hpc Hpe Hbio Hlog Hseam Hgen Hitab Hitinv
                     Hesck Hireg Hropen Hslkk Hkeep Hru Hshr Hshotc Hilink Htoken Hsbb Hsbi Hbmres Hpid
-                    Hprocs Hdev Hgeo Hdlk Hbsl Hop Hf1 Hf2 Hf3 Hf4 HbN HbW HbO
+                    Hprocs Hdev Hgeo Hdlk Hbsl Hop Htx Hf1 Hf2 Hf3 Hf4 HbN HbW HbO
                     [Hislot Hcont]").
     iEval (rewrite /wp_next).
     iIntros (CIDy) "%Hqy". iIntros (mf)
@@ -2047,6 +2053,9 @@ Section ProofSysLinkTails.
     is_lock gk d_lock "virtio_disk"%string (disk_res gd pd pav pu) -∗
     bslots 3 -∗
     log_opSe g n Sb e0 -∗
+    (* the transaction token beside the budget: this tail reaches end_op,
+       which takes the whole [log_op] (durable-disk lane A) *)
+    log_tx g -∗
     (pa_stk sp0 1) ↦₈[KT1] (m !!! Regidx Rra : mword 64) -∗
     (pa_stk sp0 2) ↦₈[KT1] (m !!! Regidx Rs0 : mword 64) -∗
     (pa_stk sp0 3) ↦₈[KT1] (m !!! Regidx Rs1 : mword 64) -∗
@@ -2078,7 +2087,7 @@ Section ProofSysLinkTails.
     iIntros "Hcg Hown #Htext #Hdata Hpc #Hpe #Hbio #Hlog Hseam Hgen #Hitab #Hitinv
               #Hesck #Hescd #Hireg #Hropen #Hslkk #Hslkd0 Hkeep Hru Hshr #Hshotc Hilink Htoken Hslkd
               Hdep Hidev Hiinum Hivalid Hload #Hshotd Hfrz Hkeepd Hrud Hsbb Hsbi
-              #Hbmres Hpid #Hprocs #Hdev #Hgeo #Hdlk Hbsl Hop Hf1 Hf2 Hf3 Hf4
+              #Hbmres Hpid #Hprocs #Hdev #Hgeo #Hdlk Hbsl Hop Htx Hf1 Hf2 Hf3 Hf4
               HbN HbW HbO Hcont".
     iDestruct (cpu_own_eb_agree with "Hcg Hown") as %Hb. cbn in Hb.
     (* ===== +0xe6 c.mv a0,s2 ===== *)
@@ -2194,7 +2203,7 @@ Section ProofSysLinkTails.
               Hlkempty Heb Hsp0 Hupsp Hupthr Hups1 Hal Hncd
               with "Hcg Hown Htext Hdata Hpc Hpe Hbio Hlog Hseam Hgen Hitab Hitinv
                     Hesck Hireg Hropen Hslkk Hkeep Hru Hshr Hshotc Hilink Htoken Hsbb Hsbi Hbmres Hpid
-                    Hprocs Hdev Hgeo Hdlk Hbsl Hop Hf1 Hf2 Hf3 Hf4 HbN HbW HbO
+                    Hprocs Hdev Hgeo Hdlk Hbsl Hop Htx Hf1 Hf2 Hf3 Hf4 HbN HbW HbO
                     [Hislot Hcont]").
     iEval (rewrite /wp_next).
     iIntros (CIDy) "%Hqy". iIntros (mf)
