iris/SpecFilewrite.v
@@ -298,7 +298,7 @@ Global Instance fwrite_names_inhabited : Inhabited fwrite_names :=
     (MkBioNames 1%positive 1%positive
        (fun _ => (1%positive, 1%positive)) (fun _ => 1%positive)
        (fun _ => 1%positive))
-    (MkLogNames 1%positive 1%positive 1%positive 1%positive)
+    (MkLogNames 1%positive 1%positive 1%positive 1%positive 1%positive)
     (MkFsNames 1%positive 1%positive 1%positive 1%positive 1%positive)
     1%positive (MkIcNames (fun _ => 1%positive) (fun _ => 1%positive)
                           (fun _ => 1%positive))
